Update gpointers

Gpointers.fst
@@ -32,11 +32,12 @@ type gnull t = (p:C.Nullity.pointer_or_null t{
   })
 
 (** Allow comparing pointers *)
-assume val g_ptr_eq:
+val g_ptr_eq:
   #a:Type ->
   p:gpointer a ->
   q:gpointer a ->
-  GTot (b:bool{b <==> (p == q)})
+  GTot (b:Type0{b <==> (p == q)})
+let g_ptr_eq #a p q = (p == q)
 
 (** Allow comparing pointers *)
 // inline_for_extraction
@@ -47,6 +48,8 @@ assume val ptr_eq:
   ST.ST bool
     (requires (fun h -> B.live h p /\ B.live h q))
     (ensures (fun h0 b h1 -> h0==h1 /\ (b <==> (g_ptr_eq p q))))
+
+let disjoint (#t:Type) (a b: gpointer t) = B.disjoint a b
 
 unfold let is_null (p:gpointer_or_null 't) = CN.is_null p
 unfold let is_not_null (p:gpointer_or_null 't) = not (CN.is_null p)
